theories/parabs/ws_hub.v
@@ -10,14 +10,14 @@ From zoo.parabs Require Export
 From zoo Require Import
   options.
 
-Implicit Types killed : bool.
-Implicit Types v t : val.
+Implicit Types b killed : bool.
+Implicit Types v t cond : val.
 
 Record ws_hub `{zoo_G : !ZooG Σ} := {
   ws_hub_create : val ;
   ws_hub_push : val ;
   ws_hub_pop : val ;
-  ws_hub_try_steal : val ;
+  ws_hub_steal_until : val ;
   ws_hub_steal : val ;
   ws_hub_killed : val ;
   ws_hub_kill : val ;
@@ -86,17 +86,21 @@ Record ws_hub `{zoo_G : !ZooG Σ} := {
       ws_hub_owner t i_
     >>> ;
 
-  ws_hub_try_steal_spec t ι i i_ max_round_noyield max_round_yield :
+  ws_hub_steal_until_spec P t ι i i_ max_round_noyield cond :
     i = Z.of_nat i_ →
     (0 ≤ max_round_noyield)%Z →
-    (0 ≤ max_round_yield)%Z →
     <<<
       ws_hub_inv t ι ∗
-      ws_hub_owner t i_
+      ws_hub_owner t i_ ∗
+      □ WP cond () {{ res,
+        ∃ b,
+        ⌜res = #b⌝ ∗
+        if b then P else True
+      }}
     | ∀∀ vs,
       ws_hub_model t vs
     >>>
-      ws_hub_try_steal t #i (#max_round_noyield, #max_round_yield)%V @ ↑ι
+      ws_hub_steal_until t #i #max_round_noyield cond @ ↑ι
     <<<
       ∃∃ o,
       match o with
@@ -108,7 +112,8 @@ Record ws_hub `{zoo_G : !ZooG Σ} := {
           ws_hub_model t vs'
       end
     | RET o;
-      ws_hub_owner t i_
+      ws_hub_owner t i_ ∗
+      if o then True else P
     >>> ;
 
   ws_hub_steal_spec t ι i i_ max_round_noyield max_round_yield :
@@ -159,7 +164,7 @@ Record ws_hub `{zoo_G : !ZooG Σ} := {
 #[global] Opaque ws_hub_create.
 #[global] Opaque ws_hub_push.
 #[global] Opaque ws_hub_pop.
-#[global] Opaque ws_hub_try_steal.
+#[global] Opaque ws_hub_steal_until.
 #[global] Opaque ws_hub_steal.
 #[global] Opaque ws_hub_killed.
 #[global] Opaque ws_hub_kill.
@@ -168,13 +173,13 @@ Section zoo_G.
   Context `{zoo_G : !ZooG Σ}.
   Context (ws_hub : ws_hub Σ).
 
-  Definition ws_hub_pop_try_steal : val :=
-    λ: "t" "i" "max_round",
+  Definition ws_hub_pop_steal_until : val :=
+    λ: "t" "i" "max_round_noyield" "cond",
       match: ws_hub.(ws_hub_pop) "t" "i" with
       | Some <> as "res" =>
           "res"
       | None =>
-          ws_hub.(ws_hub_try_steal) "t" "i" "max_round"
+          ws_hub.(ws_hub_steal_until) "t" "i" "max_round_noyield" "cond"
       end.
 
   Definition ws_hub_pop_steal : val :=
@@ -186,17 +191,21 @@ Section zoo_G.
           ws_hub.(ws_hub_steal) "t" "i" "max_round"
       end.
 
-  Lemma ws_hub_pop_try_steal_spec t ι i i_ max_round_noyield max_round_yield :
+  Lemma ws_hub_pop_steal_until_spec P t ι i i_ max_round_noyield cond :
     i = Z.of_nat i_ →
     (0 ≤ max_round_noyield)%Z →
-    (0 ≤ max_round_yield)%Z →
     <<<
       ws_hub.(ws_hub_inv) t ι ∗
-      ws_hub.(ws_hub_owner) t i_
+      ws_hub.(ws_hub_owner) t i_ ∗
+      □ WP cond () {{ res,
+        ∃ b,
+        ⌜res = #b⌝ ∗
+        if b then P else True
+      }}
     | ∀∀ vs,
       ws_hub.(ws_hub_model) t vs
     >>>
-      ws_hub_pop_try_steal t #i (#max_round_noyield, #max_round_yield)%V @ ↑ι
+      ws_hub_pop_steal_until t #i #max_round_noyield cond @ ↑ι
     <<<
       ∃∃ o,
       match o with
@@ -208,10 +217,11 @@ Section zoo_G.
           ws_hub.(ws_hub_model) t vs'
       end
     | RET o;
-      ws_hub.(ws_hub_owner) t i_
+      ws_hub.(ws_hub_owner) t i_ ∗
+      if o then True else P
     >>>.
   Proof.
-    iIntros (->) "%Hmax_round_noyield %Hmax_round_yield !> %Φ (#Hinv & Howner) HΦ".
+    iIntros (->) "%Hmax_round_noyield !> %Φ (#Hinv & Howner & #Hcond) HΦ".
 
     wp_rec.
 
@@ -222,13 +232,13 @@ Section zoo_G.
     - iRight. iExists (Some v). iFrame.
       iIntros "HΦ !> Howner". clear.
 
-      iSpecialize ("HΦ" with "Howner").
+      iSpecialize ("HΦ" with "[$Howner]").
       iSteps.
 
     - iLeft. iFrame.
-      iIntros "HΦ !> Howner". clear- Hmax_round_noyield Hmax_round_yield.
+      iIntros "HΦ !> Howner". clear- Hmax_round_noyield.
 
-      wp_smart_apply (ws_hub_try_steal_spec with "[$Hinv $Howner] HΦ"); done.
+      wp_smart_apply (ws_hub_steal_until_spec with "[$Hinv $Howner $Hcond] HΦ"); done.
   Qed.
 
   Lemma ws_hub_pop_steal_spec t ι i i_ max_round_noyield max_round_yield :
@@ -278,5 +288,5 @@ Section zoo_G.
   Qed.
 End zoo_G.
 
-#[global] Opaque ws_hub_pop_try_steal.
+#[global] Opaque ws_hub_pop_steal_until.
 #[global] Opaque ws_hub_pop_steal.
